Uniswap_v_Report.thy
@@ -1,0 +1,175 @@
+theory Uniswap_v_Report
+  imports Uniswap_v_Report_helpers
+begin
+
+section \<open>Introduction\<close>
+
+text \<open>The formalization given in this verification project is based on the Uniswap v3 whitepaper.
+
+The contract system contains 3 major modules,
+\<^item> Swapping for exchanging tokens
+\<^item> Burn \& Mint for providing and withdrawing liquidity
+\<^item> Observation for recording historical changes of the price.
+
+To the date of the document, only the first module is specified and partially verified.
+\<close>
+
+section \<open>Specifying the swap operation\<close>
+
+text \<open>
+The key concept of the swapping module is the correspondence between reserves of the two tokens,
+  the price, and the liquidity.\<close>
+
+subsection \<open>Specifying relationship between reserves, price, and liquidity\<close>
+
+text \<open>
+A key novelty of Uniswap v3 is \<^emph>\<open>virtual liquidity\<close>. Liquidity providers can limit their liquidity
+in a price interval so the amount of liquidity can be different at different price, making it a real
+function of price.
+
+To implement this, Uniswap discretizes the real function by splitting the price domain into many
+intervals named \<^emph>\<open>ticks\<close>, which are the minimal resolution unit of the price intervals of liquidity,
+so liquidity is constant in every tick.
+
+We formalize the conversion between prices and (lower bound of) ticks by \<^const>\<open>price_of\<close> and \<^const>\<open>tick_of_price\<close>,
+and lemmas @{thm price_of_tick} @{thm tick_of_price}.
+
+When the liquidity is constant in a price interval, the relation between the reserves and the price
+can be given, as the formula (6.16) and (6.13) in the whitepaper.
+
+\<open>\<Delta>x = \<Delta>(1 / sqrt(P)) * L      \<Delta>y = \<Delta>(sqrt(P)) * L\<close>
+
+We formalize this by \<^term>\<open>reserve_change_in_a_step L\<^sub>0 p\<^sub>0 p\<^sub>1\<close> which gives the change of
+the reserves of the token0 and the token1 respectively when the price moves from \<open>p\<^sub>0\<close> to \<open>p\<^sub>1\<close>,
+and when the liquidity between the prices is constant \<open>L\<^sub>0\<close>.
+\<close>
+
+lemma reserve_change_in_a_step__definition:
+  \<open>reserve_change_in_a_step L\<^sub>0 p\<^sub>0 p\<^sub>1 = (L\<^sub>0 / p\<^sub>0 - L\<^sub>0 / p\<^sub>1, L\<^sub>0 * (p\<^sub>1 - p\<^sub>0))\<close>
+  using reserve_change_in_a_step_def .
+
+text \<open>As the liquidity between two arbitrary prices is not necessarily a constant but a function of
+the price, the reserve change between the two prices is the integral over the prices, namely,
+by splitting the price interval into several partitions in every of which the liquidity is constant,
+the sum of the evaluation of the every partition.
+
+We formalize this by \<^const>\<open>Const_Interval\<close>, \<^const>\<open>Is_partition\<close>, and \<^const>\<open>partition_intergral\<close>.
+\<close>
+
+lemma Const_Interval__definition:
+  \<open>Const_Interval L\<^sub>p l u \<longleftrightarrow> l \<le> u \<and> (\<forall>k. l \<le> k \<and> k < u \<longrightarrow> L\<^sub>p k = L\<^sub>p l)\<close>
+  unfolding Const_Interval_def by (smt (verit, best)) 
+
+text \<open>\<^term>\<open>L\<^sub>p :: price \<Rightarrow> liquidity\<close> is the function from prices to their liquidity.
+Predicate \<^term>\<open>Const_Interval L\<^sub>p l u\<close> specifies \<open>[l,u)\<close> is a price interval where the liquidity
+on the prices is constant.\<close>
+
+lemma Is_partition__definition:
+  \<open>Is_partition L\<^sub>p l u [] \<longleftrightarrow> Const_Interval L\<^sub>p l u\<close>
+  \<open>Is_partition L\<^sub>p l u ([h] + r) \<longleftrightarrow> Const_Interval L\<^sub>p l h \<and> Is_partition L\<^sub>p h u r\<close>
+  by simp+
+
+text \<open>We use an order list (a chain) to represent a partition, e.g. \<^term>\<open>[x\<^sub>0,x\<^sub>1,x\<^sub>2]\<close> for \<open>[l,x\<^sub>0), [x\<^sub>0,x\<^sub>1), [x\<^sub>1,x\<^sub>2), [x\<^sub>2,u)\<close>.
+Predicate \<open>Is_partition f l u ps\<close> asserts if \<open>ps\<close> is a valid partition where every interval has constant liquidity.
+
+Then, we can add up the evaluation of every partition to get the integral, by a recursion function as the following.
+\<close>
+
+lemma partition_intergral__definition:
+  \<open>partition_intergral reserve_change_in_a_step L\<^sub>p low up []
+      = reserve_change_in_a_step (L\<^sub>p low) low up\<close>
+  \<open>partition_intergral reserve_change_in_a_step L\<^sub>p low up ([h] + r)
+      = reserve_change_in_a_step (L\<^sub>p low) low h + partition_intergral reserve_change_in_a_step L\<^sub>p h up r\<close>
+  by simp+
+
+
+text \<open>Finally, we can specify the relationship between reserves, price, and liquidity,
+  which is the integral following any valid partition.\<close>
+
+lemma
+\<open>reserve_change' L lower upper
+    = partition_intergral reserve_change_in_a_step (L \<circ> tick_of_price) lower upper
+                          (SOME ps. Is_partition (L \<circ> tick_of_price) lower upper ps)\<close>
+  by (metis Eps_cong Is_key_partition_implies_Is_partition reserve_change'_def reserve_change_irrelavent_with_partition someI_ex)
+
+text \<open>\<^term>\<open>L :: tick \<Rightarrow> liquidity\<close> is the function from ticks to their liquidity.
+There is \<open>L \<circ> tick_of_price \<equiv> L\<^sub>p\<close>.
+By lemma @{thm partition_intergral_irrelavent_with_parition}, the result of the integral is irrelavent
+with specific partitions.\<close>
+
+text \<open>Now we can specify the swap operation of Uniswap.\<close>
+
+subsection \<open>Specifying swap operation\<close>
+
+lemma (in Pool)
+ \<open>\<p>\<r>\<e>\<m>\<i>\<s>\<e> 0 \<noteq> amount_specified \<and> 0 < price_limit \<Longrightarrow>
+  \<p>\<r>\<e>\<m>\<i>\<s>\<e> unlocked \<Longrightarrow>
+  \<p>\<r>\<e>\<m>\<i>\<s>\<e> (if zeroForOne then price_limit < price \<and> MIN_PRICE < price_limit else price < price_limit \<and> price_limit < MAX_PRICE) \<Longrightarrow>
+
+  \<p>\<r>\<o>\<c> swap (\<a>\<r>\<g>3 \<^bold>, \<a>\<r>\<g>2 \<^bold>, \<a>\<r>\<g>1)
+  \<lbrace> (price, i, unlocked, Lg, L, growth, \<delta>, fee_protocol, protocal_fees) \<Ztypecolon> Uniswap_Pool\<heavy_comma>
+     zeroForOne \<Ztypecolon> \<v>\<a>\<l>[\<a>\<r>\<g>1] \<bool>\<heavy_comma> amount_specified \<Ztypecolon> \<v>\<a>\<l>[\<a>\<r>\<g>2] \<real>\<heavy_comma> price_limit \<Ztypecolon> \<v>\<a>\<l>[\<a>\<r>\<g>3] \<real>
+  \<longmapsto>
+   (price', i', unlocked, Lg, L, growth + fee_growth zeroForOne fee_factor L price price', \<delta>, fee_protocol,
+       protocal_fees + \<Delta>protocal_fees fee_protocol zeroForOne L price price' fee_factor) \<Ztypecolon> Uniswap_Pool\<heavy_comma>
+     transfer_out \<Ztypecolon> \<v>\<a>\<l> \<real>\<heavy_comma> transfer_in \<Ztypecolon> \<v>\<a>\<l> \<real>
+   \<s>\<u>\<b>\<j> price' i' transfer_out transfer_in.
+     (if zeroForOne then price_limit \<le> price' else price' \<le> price_limit) \<and>
+     (price' = price_limit \<or>
+      (if 0 < amount_specified then amount_specified * (1 - fee) = (if zeroForOne then fst else snd) (reserve_change zeroForOne L price price')
+       else - amount_specified = (if zeroForOne then snd else fst) (reserve_change zeroForOne L price price'))) \<and>
+     transfer_out = (if zeroForOne then snd else fst) (reserve_change zeroForOne L price price') \<and>
+     transfer_in = (if zeroForOne then fst else snd) (reserve_change zeroForOne L price price') / (1 - fee)
+  \<rbrace>\<close>
+  using swap_\<phi>app .
+
+text \<open>Right now we have only verified the operation works correctly when the input arguments are valid as
+  specified in the three leading premises. When our underlying verification platform is completed,
+  we can in addition show a state revert would happen on invalid arguments so completes
+  this verification.
+
+The proof is given by theorem @{thm Uniswap_Pool.Pool.swap_\<phi>app}.
+
+Argument \<^term>\<open>zeroForOne\<close> indicates if the user wants to buy token1 using token0 or reversely.
+\<^term>\<open>amount_specified\<close> is the amount that the user wants to pay if it is positive,
+or the amount that user wants to pay for if it is negative.
+As the transaction affects the price, the transaction terminates once the price reaches the \<^term>\<open>price_limit\<close>
+or all the specified amount is processed.
+
+The initial state of the Uniswap pool contract is on price \<^term>\<open>price\<close>, tick \<^term>\<open>i\<close>, liquidity \<^term>\<open>L\<close>.
+\<^term>\<open>growth :: tick \<Rightarrow> fee \<times> fee\<close> is the function from ticks to transaction fees that have been
+gained on the tick, in earning per unit of liquidity and for token0 and token1 respectively.
+Liquidity providers' yields are calculated by multiplying it by the amount of their liquidity.
+\<^term>\<open>fee_protocol\<close> is the proportion of the contract owner's commission from the transaction fee.
+\<^term>\<open>protocal_fees\<close> is the amount of the contract owner's commission that has been gained.
+
+\<^term>\<open>Lg\<close> is a technical scaffold used in the implementation. So-called \<^emph>\<open>Gross Liquidity\<close>, it is
+a function from ticks to the total amount of liquidity providers' intervals that reference the tick.
+
+The above lemma specifies, after execution of the swap operation, the resulted price \<^term>\<open>price'\<close>
+will either reaches the \<^term>\<open>price_limit\<close> (but never exceeds it), or, is exactly the one causing
+that the reserve change equals to the specified amount, with transaction fee considered.
+\<open>reserve_change zeroForOne L price next_price \<equiv> (if zeroForOne then reserve_change' L next_price price else reserve_change' L price next_price)\<close>
+\<^term>\<open>reserve_change\<close> is precisely the \<^term>\<open>reserve_change'\<close> defined above but just considers the
+order of the prices (buying token1 using token0 causes the price decreases and reversely for the other side).
+
+The amount \<^term>\<open>transfer_in\<close> that the user needs to pay and \<^term>\<open>transfer_out\<close> that Uniswap transfers to the user
+are the change of the reserves, with consideration of transaction fee.
+
+\<^const>\<open>fee\<close> is the rate of the transaction fee.
+The record of the transaction fees is increased by \<open>fee_growth zeroForOne fee_factor L price price'\<close>
+which gives for each tick the the fee per liquidity of the transaction moving the price from \<^term>\<open>price\<close> to \<^term>\<open>price'\<close>.
+Note both \<^term>\<open>growth\<close> and \<^term>\<open>fee_growth zeroForOne fee_factor L price price'\<close> are functions of ticks,
+and the addition is defined pointwisely.
+\<^term>\<open>\<Delta>protocal_fees fee_protocol zeroForOne L price price' fee_factor\<close> gives the fee of
+the contract owner's commission accordingly.
+
+To conclude, we have verified the proper behavior of the swap operation under valid input arguments.
+We haven't considered arithmetic overflow and precision error of fix-point arithmetic.
+The verification is done on an abstract specification level where we use variables instead of
+the exact solidity semantics to formalize the program.
+We will keep developing our framework to cover the complete Uniswap modules, complete argument domain,
+and concrete solidity semantics.
+\<close>
+
+end
