ROOT
@@ -1,0 +1,9 @@
+session Uniswap_v = "Phi_Semantics" +
+  theories
+    Uniswap_Pool
+    Uniswap_SqrtPriceMath
+    Uniswap_Tick
+    Uniswap_Tick_Math
+    Uniswap_TickBitmap
+    Uniswap_v_Report_helpers
+    Uniswap_v_Report
